---
created: 250424 14:18:11
updated: 250424 14:18:12
---
1. if `a` and `b` are in the group, then `a + b` is also in the group
2. `(a + b) + c = a + (b + c)`
3. there exists an element 0 such that `a + 0 = a`
4. for every `a`, there exists `-a` such that `a + (-a) = 0`

group `A` is additive and `a, b, c` is an element of `A`.
If `a, b, c` are identical each other,

$$
a + b \ne a + c
$$

Assume that 

$$
a + b = a + c
$$

From constraint `A` is additive group, there exist `-a` and

$$
a + (-a) + b = a + (-a) + c
$$
this leads to

$$
b = c
$$

but `b, c` are identical, then

$$
a + b \ne a + c
$$

is true